README.md
@@ -2,3 +2,8 @@ lazyKoq
 =======
 
 interpreter of lazy K written by Coq
+
+TODO:
+1. function of (lambda formula TO combinator)
+2. function of (string TO Church number)
+3. function of (Church number TO string)
